Foundation/ProvabilityLogic/Kripke/FiniteLineModel.lean
@@ -31,12 +31,12 @@ lemma rank_eq (x : (finiteLineModel n α).World) : x.rank = x := by
   induction k using Nat.strong_induction_on with
   | h k ih =>
     apply le_antisymm;
-    . apply cwfHeight_le;
+    · apply cwfHeight_le;
       rintro ⟨l, hl⟩ (h : l < k);
       exact (ih l h hl).trans_lt h;
-    . rcases k with _ | k;
-      . simp;
-      . have h : (finiteLineModel n α).Rel ⟨k + 1, hk⟩ ⟨k, by omega⟩ := Nat.lt_add_one k;
+    · rcases k with _ | k;
+      · simp;
+      · have h : (finiteLineModel n α).Rel ⟨k + 1, hk⟩ ⟨k, by omega⟩ := Nat.lt_add_one k;
         have := rank_lt_of_rel h;
         rw [ih k (by omega) (by omega)] at this;
         exact this;
