Foundation/ProvabilityLogic/S/Boxdot.lean
@@ -20,12 +20,12 @@ variable {α : Type u} [DecidableEq α] {A : Formula α}
 
 theorem boxdotTranslate_iff_GL : 𝐒 ⊢ Aᵇ ↔ 𝐆𝐋 ⊢ Aᵇ := by
   constructor;
-  . intro h;
+  · intro h;
     apply GL.iff_root_forces.mpr;
     intro _ _ M _;
     obtain ⟨i, hi⟩ := iff_eventually_forces_tail.mp h M;
     exact (RootedModel.toTail.forces_inr_boxdotTranslate_iff i).mp (hi i le_rfl);
-  . exact of_GL;
+  · exact of_GL;
 
 end Logic.S
 
